parse_list_impl

examples/miniparse/MiniParse.Impl.List.fst
@@ -4,14 +4,212 @@ include MiniParse.Impl.Base
 
 module U8 = FStar.UInt8
 module U32 = FStar.UInt32
+module HS = FStar.HyperStack
+module HST = FStar.HyperStack.ST
+module B = LowStar.Buffer
+module BO = LowStar.BufferOps
+module M = LowStar.ModifiesPat
+module CL = C.Loops
+module L = FStar.List.Tot
 
-assume val parse_nlist_impl
+let parse_nlist_impl_inv_easy
+  (#t: Type0)
+  (n: nat)
+  (h0: HS.mem)
+  (b: buffer8)
+  (rb: B.pointer (x: U32.t { U32.v x <= B.length b } ))
+  (rr: B.pointer (list t))
+  (h: HS.mem)
+  (i: nat)
+  (stop: bool)
+: Tot Type0
+= M.loc_disjoint (M.loc_buffer rb) (M.loc_buffer rr) /\
+  M.loc_disjoint (M.loc_buffer b) (M.loc_union (M.loc_buffer rb) (M.loc_buffer rr)) /\
+  M.modifies (M.loc_union (M.loc_buffer rb) (M.loc_buffer rr)) h0 h /\
+  i <= n /\
+  B.live h0 b /\ B.live h b /\ B.live h rb /\ B.live h rr
+
+let parse_nlist_impl_inv
+  (#t: Type0)
+  (p0: parser_spec t)
+  (n: nat)
+  (h0: HS.mem)
+  (b: buffer8)
+  (rb: B.pointer (x: U32.t { U32.v x <= B.length b } ))
+  (rr: B.pointer (list t))
+  (h: HS.mem)
+  (i: nat)
+  (stop: bool)
+: Tot Type0
+= parse_nlist_impl_inv_easy n h0 b rb rr h i stop /\ (
+  let off = BO.deref h rb in
+  let b' = B.gsub b off (B.len b `U32.sub` off) in
+  let p = parse (parse_nlist n p0) (B.as_seq h0 b) in
+  let p' = parse (parse_nlist (n - i) p0) (B.as_seq h0 b') in
+  if stop
+  then None? p
+  else match p, p' with
+  | Some (l, consumed), Some (l', consumed') ->
+    consumed == U32.v off + consumed' /\
+    l == L.append (L.rev (BO.deref h rr)) l'
+  | None, None -> True
+  | _ -> False
+  )
+
+let list_assoc_append (#t: Type) (x: t) (l1 l2: list t) : Lemma
+  (L.append (L.rev l1) (x :: l2) == L.append (L.rev (x :: l1)) l2)
+= L.append_assoc (L.rev l1) [x] l2;
+  L.rev_append [x] l1
+
+#set-options "--z3rlimit 64 --max_ifuel 8"
+
+let parse_nlist_impl_inv_false_intro
+  (#t: Type0)
+  (p0: parser_spec t)
+  (n: nat)
+  (h0: HS.mem)
+  (b: buffer8)
+  (rb: B.pointer (x: U32.t { U32.v x <= B.length b } ))
+  (rr: B.pointer (list t))
+  (h1 h2: HS.mem)
+  (i: nat { i < n } )
+  (off : U32.t)
+  (off' : U32.t)
+  (b' : buffer8)
+  (b'_after : buffer8)
+  (l: nlist n t)
+  (elem: t)
+  (consumed1: nat)
+  (consumed: nat)
+  (l'_before: nlist (n - i) t)
+  (consumed_before : nat)
+  (l'_after: nlist (n - (i + 1)) t)
+  (consumed_after: nat)
+: Lemma
+  (requires (
+    parse_nlist_impl_inv p0 n h0 b rb rr h1 (i) false /\
+    parse_nlist_impl_inv_easy n h0 b rb rr h2 (i + 1) false /\
+    off == BO.deref h1 rb /\
+    off' == BO.deref h2 rb /\
+    U32.v off' == U32.v off + consumed1 /\
+    b' == B.gsub b off (B.len b `U32.sub` off) /\
+    b'_after == B.gsub b off' (B.len b `U32.sub` off') /\
+    consumed <= Seq.length (B.as_seq h0 b) /\
+    parse (parse_nlist (n) p0) (B.as_seq h0 b) == Some (l, consumed) /\
+    consumed1 <= Seq.length (B.as_seq h0 b') /\
+    parse p0 (B.as_seq h0 b') == Some (elem, consumed1) /\
+    consumed_before <= Seq.length (B.as_seq h0 b') /\
+    parse (parse_nlist (n - i) p0) (B.as_seq h0 b') == Some (l'_before, consumed_before) /\
+    consumed_after <= Seq.length (B.as_seq h0 b'_after) /\
+    parse (parse_nlist (n - (i + 1)) p0) (B.as_seq h0 b'_after) == Some (l'_after, consumed_after) /\
+    BO.deref h2 rr == elem :: BO.deref h1 rr /\
+    True
+  ))
+  (ensures (
+    parse_nlist_impl_inv p0 n h0 b rb rr h2 (i + 1) false
+  ))
+= parse_nlist_eq (n - i) p0 (B.as_seq h0 b');
+  assert (b'_after == B.gsub b' (U32.uint_to_t consumed1) (B.len b `U32.sub` off'));
+  assert (consumed == U32.v off + consumed_before);
+  let l1 = BO.deref h1 rr in
+  assert (l == L.append (L.rev l1) l'_before);
+  assert (consumed == U32.v off' + consumed_after);
+  assert (l'_before == elem :: l'_after);
+  list_assoc_append elem l1 l'_after;
+  assert (l == L.append (L.rev (elem :: l1)) l'_after);
+  assert (parse_nlist_impl_inv p0 n h0 b rb rr h2 (i + 1) false)
+
+// (parse (parse_nlist (n + 1) p) b == match parse (parse_nlist n
+
+inline_for_extraction
+val parse_nlist_impl_body
+  (#t: Type0)
+  (p0: parser_spec t)
+  (pimpl: parser_impl p0)
+  (n: nat)
+  (h0: HS.mem)
+  (b: buffer8)
+  (len: U32.t { len == B.len b } )
+  (rb: B.pointer (x: U32.t { U32.v x <= B.length b } ))
+  (rr: B.pointer (list t))
+  (i: U32.t { 0 <= U32.v i /\ U32.v i < n } )
+: HST.Stack bool
+  (requires (fun h -> parse_nlist_impl_inv p0 n h0 b rb rr h (U32.v i) false))
+  (ensures (fun h res h' ->
+    parse_nlist_impl_inv p0 n h0 b rb rr h (U32.v i) false /\
+    parse_nlist_impl_inv p0 n h0 b rb rr h' (U32.v i + 1) res
+  ))
+
+let parse_nlist_impl_body #t p0 pimpl n h0 b len rb rr i =
+  let off = BO.op_Bang_Star rb in
+  let b' = B.offset b off in
+  assert (n - U32.v i > 0);
+  let h = HST.get () in
+  let h1 = h in
+  match pimpl b' (len `U32.sub` off) with
+  | None ->
+    true
+  | Some (elem, consumed) ->
+    assert (let (Some (elem', consumed')) = parse p0 (B.as_seq h b') in elem == elem' /\ U32.v consumed == consumed');
+    assert (U32.v consumed <= U32.v (len `U32.sub` off));
+    let off' = off `U32.add` consumed in
+    assert (len `U32.sub` off' == B.len b' `U32.sub` consumed);
+    B.gsub_gsub b off (len `U32.sub` off) consumed (len `U32.sub` off');
+    BO.op_Star_Equals rb off';
+    let l1 = BO.op_Bang_Star rr in
+    BO.op_Star_Equals rr (elem :: l1);
+    let h = HST.get () in
+//    assume (M.modifies (M.loc_union (M.loc_buffer rb) (M.loc_buffer rr)) h0 h);
+    assert (parse_nlist_impl_inv_easy n h0 b rb rr h (U32.v i + 1) false);
+    parse_nlist_eq (n - U32.v i) p0 (B.as_seq h0 b');
+    let phi () : Lemma (parse_nlist_impl_inv p0 n h0 b rb rr h (U32.v i + 1) false) =
+      let p = parse (parse_nlist n p0) (B.as_seq h0 b) in
+      let i = U32.v i in
+      let b'_after = B.gsub b off' (len `U32.sub` off') in
+      assert (off' == BO.deref h rb);
+      assert (b'_after == B.gsub b off' (B.len b `U32.sub` off'));
+      let p'_before = parse (parse_nlist (n - i) p0) (B.as_seq h0 b') in
+      let p'_after = parse (parse_nlist (n - (i + 1)) p0) (B.as_seq h0 b'_after) in
+      assert (None? p == None? p'_before);
+      assert (b'_after == B.gsub b' consumed (len `U32.sub` off'));
+      assert (None? p'_before == None? p'_after);
+      let consumed1 = U32.v consumed in
+      match p, p'_before, p'_after with
+      | Some (l, consumed), Some (l'_before, consumed'_before), Some (l'_after, consumed'_after) ->
+        parse_nlist_impl_inv_false_intro p0 n h0 b rb rr h1 h i off off' b' b'_after l elem consumed1 consumed l'_before consumed'_before l'_after consumed'_after
+      | _ -> ()
+    in
+    phi ();
+    false
+
+inline_for_extraction
+let parse_nlist_impl
   (n: nat)
   (n' : U32.t { U32.v n' == n } )
   (#t: Type0)
   (#p: parser_spec t)
   (p32: parser_impl p)
 : Tot (parser_impl (parse_nlist n p))
+= fun b len ->
+  HST.push_frame ();
+  let rr : B.pointer (list t) = B.alloca [] 1ul in
+  let rb : B.pointer (x: U32.t { U32.v x <= B.length b } ) = B.alloca 0ul 1ul in
+  let h0 = HST.get () in
+  let (_, stop) =
+    CL.interruptible_for 0ul n'
+      (parse_nlist_impl_inv p n h0 b rb rr)
+      (parse_nlist_impl_body p p32 n h0 b len rb rr)
+  in
+  let l = BO.op_Bang_Star rr in
+  let consumed = BO.op_Bang_Star rb in
+  let res : option (nlist n t * U32.t) =
+    if stop
+    then None
+    else Some (L.rev l, consumed)
+  in
+  HST.pop_frame ();
+  res
+
 
 assume val serialize_nlist_impl
   (n: nat)
